update

Jrlean/Relation.lean
@@ -2,4 +2,10 @@ module
 
 namespace Jrlean
 
-public abbrev Relation (α : Sort u) := α → α → Prop
+public abbrev Relation (α : Sort u) (β : Sort v) := α → β → Prop
+
+@[grind, expose]
+public def Relation.rev (r : Relation α β) : Relation β α := fun b a => r a b
+
+@[simp, grind =]
+public theorem rev_rev (r : Relation α β) : r.rev.rev = r := by grind only [Relation.rev]
