Jrlean/Assumption.lean
@@ -1,0 +1,8 @@
+module
+
+namespace Jrlean
+
+public meta section
+
+/-- Just calls the `assumption` tactic -/
+macro stx:"assumption" : term => `(by assumption%$stx)
