Jrlean/Coc.lean
@@ -6,6 +6,7 @@ public import Jrlean.Coc.Notation
 public import Jrlean.Coc.Repr
 public import Jrlean.Coc.MoveIntoOutOf
 public import Jrlean.Coc.Beta
+public import Jrlean.Coc.BetaHeadInduction
 public import Jrlean.Coc.BetaLemmas
 public import Jrlean.Coc.Logical
 public import Jrlean.Coc.LogicalLemmas
