Jrlean/Coc/BetaHeadInduction.lean
@@ -1,0 +1,133 @@
+module
+
+public import Jrlean.Coc.Beta
+public import Jrlean.SetTactic
+
+namespace Jrlean.Coc.Term
+
+@[elab_as_elim]
+public theorem betaHeadInduction
+[VarKind]
+{motive : Term → Prop}
+(prop : motive prop)
+(type : motive type)
+(var : ∀ v, motive (var v))
+(binder : ∀ k v ty body, motive ty → motive body → motive (binder k v ty body))
+(app : ∀ f a, betaHead (app f a) = none → motive f → motive a → motive (app f a))
+(betaHead : ∀ v ty body arg, motive ty → motive body → motive (.app (lam v ty body) arg))
+t
+: motive t := by
+  -- To prove the goal, we need induction, but over a stronger proposition
+  suffices motive t ×' match t with
+    -- we carry the proof of the inductive hypothesis of the type and body too
+    | .binder k v ty body => motive ty ×' motive body
+    | _ => PUnit from this.1
+  induction t
+  -- Cases where t is prop, type or var are very simple.
+  iterate 3 constructor; apply_assumption; exact .unit
+  -- In the binder case, we carry the inductive hypotheses
+  case binder k v ty body ih_ty ih_body =>
+    exact ⟨binder k v ty body ih_ty.1 ih_body.1, ih_ty.1, ih_body.1⟩
+  -- In the application case, we match on the lhs, and if it's a function, we use the betaHead
+  -- lemma to solve it, otherwise we use the app case.
+  case app f a ih_f ih_a =>
+    -- Just need to prove the induction hypothesis, nothing else
+    suffices motive (.app f a) from ⟨this, .unit⟩
+    -- Clean the context
+    clear binder type prop var
+    cases f
+    case' binder k v ty body =>
+      cases k
+      case lam =>
+        -- This is the only case where we have a beta head
+        obtain ⟨_, ih_ty, ih_body⟩ := ih_f
+        exact betaHead v ty body a ih_ty ih_body
+    -- In all other, regular recursion
+    all_goals apply app _ a rfl ih_f.1 ih_a.1
+
+@[elab_as_elim]
+public theorem betaHeadInduction'
+[VarKind]
+{motive : Term → Prop}
+(prop : motive prop)
+(type : motive type)
+(var : ∀ v, motive (var v))
+(binder : ∀ k v ty body, motive ty → motive body → motive (binder k v ty body))
+(app : ∀ f a, betaHead (app f a) = none → motive f → motive a → motive (app f a))
+(betaHead : ∀ v ty body arg, motive (body.moveOutOfBinder v.toVar arg)
+  → motive (.app (lam v ty body) arg))
+t
+: motive t := by
+  -- To prove the goal, we need induction, but over a stronger proposition
+  suffices motive t ×' match t with
+    -- we carry the proof of the inductive hypothesis of the type and body too
+    | .binder k v ty body => motive ty ×' motive body
+    | _ => PUnit from this.1
+  induction t
+  -- Cases where t is prop, type or var are very simple.
+  iterate 3 constructor; apply_assumption; exact .unit
+  -- In the binder case, we carry the inductive hypotheses
+  case binder k v ty body ih_ty ih_body =>
+    exact ⟨binder k v ty body ih_ty.1 ih_body.1, ih_ty.1, ih_body.1⟩
+  -- In the application case, we match on the lhs, and if it's a function, we use the betaHead
+  -- lemma to solve it, otherwise we use the app case.
+  case app f a ih_f ih_a =>
+    -- Just need to prove the induction hypothesis, nothing else
+    suffices motive (.app f a) from ⟨this, .unit⟩
+    -- Clean the context
+    clear binder type prop var
+    cases f
+    case' binder k v ty body =>
+      cases k
+      case lam =>
+        -- This is the only case where we have a beta head
+        obtain ⟨_, ih_ty, ih_body⟩ := ih_f
+        exact betaHead v ty body a ih_ty ih_body
+    -- In all other, regular recursion
+    all_goals apply app _ a rfl ih_f.1 ih_a.1
+
+Jrlean.Coc.Term.BetaEquiv.recOn
+[varKind : VarKind]
+{motive : (a a_1 : Term) → a =β a_1 → Prop}
+{a✝ a✝¹ : Term}
+(t : a✝ =β a✝¹)
+(beta : ∀ {x : VarDecl} {ty body arg : Term}, motive ((lam x ty body).app arg) (body.moveOutOfBinder x.toVar arg) ⋯)
+(refl : ∀ {t : Term}, motive t t ⋯) (symm : ∀ {t₁ t₂ : Term} (a : t₁ =β t₂), motive t₁ t₂ a → motive t₂ t₁ ⋯)
+(trans : ∀ {t₁ t₂ t₃ : Term} (a : t₁ =β t₂) (a_1 : t₂ =β t₃), motive t₁ t₂ a → motive t₂ t₃ a_1 → motive t₁ t₃ ⋯)
+(app_congr :
+  ∀ {f₁ f₂ a₁ a₂ : Term} (a : f₁ =β f₂) (a_1 : a₁ =β a₂),
+    motive f₁ f₂ a → motive a₁ a₂ a_1 → motive (f₁.app a₁) (f₂.app a₂) ⋯)
+(binder_congr :
+  ∀ {k : BinderKind} {v : VarDecl} {ty₁ ty₂ body₁ body₂ : Term} (a : ty₁ =β ty₂) (a_1 : body₁ =β body₂),
+    motive ty₁ ty₂ a → motive body₁ body₂ a_1 → motive (binder k v ty₁ body₁) (binder k v ty₂ body₂) ⋯) :
+motive a✝ a✝¹ t
+
+@[elab_as_elim]
+public theorem inductionWithoutTrans
+[VarKind]
+{motive : Term → Term → Prop}
+(t₁ t₂ : Term)
+(h_equiv : t₁ =β t₂)
+(beta : ∀ v ty t₁ t₂ arg, motive t₁ t₂ → motive (.app (.lam v ty t₁) arg) (t₁.moveOutOfBinder v.toVar arg))
+(refl : ∀ t, motive t t)
+(symm : ∀ t₁ t₂, motive t₁ t₂ → motive t₂ t₁)
+(app : ∀ f₁ f₂ a₁ a₂, motive f₁ f₂ → motive a₁ a₂ → motive (.app f₁ a₁) (.app f₂ a₂))
+(binder : ∀ k v ty₁ ty₂ body₁ body₂, motive ty₁ ty₂ → motive body₁ body₂
+  → motive (.binder k v ty₁ body₁) (.binder k v ty₂ body₂))
+: motive t₁ t₂ := by
+  suffices motive t₁ t₂ ∧ ∀ t₃, (motive t₂ t₃ → motive t₁ t₃) ∧ (motive t₁ t₃ → motive t₂ t₃)
+  from this.1
+  induction h_equiv
+  case beta v ty body arg =>
+    apply And.intro
+    · apply beta (t₁:=body) (t₂:=body)
+      apply refl
+    · intro t₃
+      apply And.intro
+      · intro h_t₃
+        induction t₃
+        case type => 
+  case refl => apply refl
+  case symm => apply symm; assumption
+  case trans t₁ t₂ t₃ h₁ h₂ ih₁ ih₂ =>
+
