Jrlean/Confluence.lean
@@ -1,0 +1,46 @@
+module
+
+public import Jrlean.Relation
+public import Jrlean.ReflexiveTransitiveClosure
+public import Jrlean.Diamond
+public import Init
+
+namespace Jrlean
+
+public section
+
+/-!
+A confluence property is a generalization of the `Diamond` property.
+-/
+class abbrev Confluence (r : Relation α α) := Diamond (r*)
+
+namespace Confluence
+
+variable {α : Sort u} {r : Relation α α}
+
+theorem of_diamond : Diamond r → Confluence r := by
+  intro instDiamond
+  -- First we prove a smaller statement.
+  have aux : ∀ a b c, (r*) a b → r a c → ∃ d, r b d ∧ (r*) c d := by
+    intro a b c h_a_b h_a_c
+    induction h_a_b using ReflTransClosure.rightInduction
+    case refl a => grind
+    case rightCons a b₁ b₂ h_a_b₁ h_b₁_b₂ ih =>
+      -- We need to find the `d`, and it happens to be the one from the diamond property with the
+      -- induction hypothesis's `d`.
+      have ⟨d, h_b₁_d, h_c_d⟩ := ih h_a_c; clear ih h_a_c
+      have ⟨e, h_b₂_e, h_d_e⟩ := Diamond.diamond b₁ b₂ d h_b₁_b₂ h_b₁_d
+      have h_c_e : (r*) c e := h_c_d.rightCons h_d_e
+      exact ⟨e, h_b₂_e, h_c_e⟩
+  -- Now comes the main part
+  suffices Diamond (r*) from .mk
+  constructor; intro a b c h_a_b h_a_c
+  -- In the lemma at the start, we did induction on `h_a_b`. Now we do on the other one.
+  induction h_a_c using ReflTransClosure.rightInduction
+  case refl a => exists b
+  case rightCons a c₁ c₂ h_a_c₁ h_c₁_c₂ ih =>
+    have ⟨d, h_b_d, h_c₁_d⟩ := ih assumption
+    have ⟨e, h_d_e, h_c₂_e⟩ := aux c₁ d c₂ assumption assumption
+    exact ⟨e, h_b_d.rightCons h_d_e, h_c₂_e⟩
+
+instance [Diamond r] : Confluence r := .of_diamond inferInstance
