Jrlean/Diamond.lean
@@ -1,0 +1,14 @@
+module
+
+public import Jrlean.Relation
+
+namespace Jrlean
+
+public section
+
+/--
+A proof that a relation sort of comes back together.
+This is similiar to `Confluence`, and is useful for proving it.
+-/
+class Diamond (r : Relation α α) where
+  diamond : ∀ a b c, r a b → r a c → ∃ d, r b d ∧ r c d
