Jrlean/ReflexiveTransitiveClosure.lean
@@ -1,0 +1,124 @@
+module
+
+public import Jrlean.Relation
+public import Jrlean.Subrelation
+public import Jrlean.Assumption
+meta import Lean
+
+namespace Jrlean
+
+public section
+
+-- First let's start with defining names and notation
+
+variable {α : Sort u}
+
+@[grind]
+inductive ReflTransClosure (r : Relation α α) : Relation α α where
+| refl {a} : ReflTransClosure r a a
+| leftCons : r a b → ReflTransClosure r b c → ReflTransClosure r a c
+
+-- We also have the full name
+abbrev ReflexiveTransitiveClosure (r : Relation α α) := ReflTransClosure r
+
+postfix:max "*" => ReflTransClosure
+
+-- Now let's define lemmas
+
+namespace ReflTransClosure
+
+variable {r : Relation α α}
+variable {a b c : α}
+
+section Refl
+
+attribute [refl] refl
+
+instance : Std.Refl r* where refl _ := refl
+
+end Refl
+
+section Trans
+
+@[grind →, grind <=, grind .]
+theorem trans : (r*) a b → (r*) b c → (r*) a c := by
+  intro left right
+  induction left <;> grind
+
+@[grind .]
+theorem rightCons : (r*) a b → r b c → (r*) a c := by grind
+
+instance instTrans : Trans (r*) (r*) (r*) where trans := trans
+instance instTransLeftCons : Trans r (r*) (r*) where trans := leftCons
+instance instTransRightCons : Trans (r*) r (r*) where trans := rightCons
+
+end Trans
+
+section Symm
+
+@[symm, grind .]
+theorem symm_of_symm [Std.Symm r] : (r*) a b → (r*) b a := by
+  intro h
+  induction h
+  case refl => trivial
+  case leftCons a₁ a₂ b head tail ih =>
+    replace head := Std.Symm.symm _ _ head
+    grind
+
+end Symm
+
+@[grind →]
+theorem eq_of_subrelation_of_subrelation {r₁ r₂ : Relation α α}
+: r₁ ⊆ r₂ → r₂ ⊆ r₁* → r₂* = r₁* := by
+  intro h₁ h₂
+  symm
+  two_directions
+  case forward =>
+    constructor; intro a b h_r₁_star
+    show (r₂*) a b
+    induction h_r₁_star <;> grind
+  case backward =>
+    constructor; intro a b h_r₂_star
+    show (r₁*) a b
+    induction h_r₂_star <;> grind
+
+section Reverse
+
+@[simp, grind =]
+theorem rev_eq_rev : (r*).rev = r.rev* := by
+  two_directions
+  all_goals constructor; intro a b h
+  case forward =>
+    induction h
+    case refl => trivial
+    case leftCons => grind only [rightCons, = Relation.rev.eq_1]
+  case backward =>
+    induction h
+    case refl => sorry
+    case leftCons => grind only [= Relation.rev.eq_1, rightCons]
+
+end Reverse
+
+@[elab_as_elim]
+theorem rightInduction
+{motive : ∀ a b, (r*) a b → Prop}
+(h : (r*) a b)
+(refl : ∀ a, motive a a .refl)
+(rightCons : ∀ (a b c : α) h₁ h₂, motive a b h₁ → motive a c (.rightCons h₁ h₂))
+: motive a b h := by
+  -- We construct the proof from the right using left induction by switching the order of the
+  -- arguments and using left induction. In order to do that, we define an reversed relation.
+  let r' := r.rev
+  rename (r*) a b => h_old
+  have h : (r'*) b a := by sorry
+  -- Induction on the reversed proof of (r*)!
+  induction h
+  case refl a => apply refl
+  case leftCons b₂ b₁ a head tail ih =>
+    have : (r*) a b₁ := by sorry
+    have : r b₁ b₂ := head
+    have : motive a b₁ assumption := by sorry
+    apply rightCons a b₁ b₂ <;> assumption
+
+@[grind <=]
+theorem singleton : r a b → (r*) a b := fun x => .leftCons x .refl
