Jrlean/Subrelation.lean
@@ -1,0 +1,28 @@
+module
+
+public import Jrlean.Relation
+
+namespace Jrlean
+
+public section
+
+variable {α : Sort u} {β : Sort v}
+variable {r r₁ r₂ r₃ : Relation α β}
+
+/-- Is the left relation a subrelation of the right one? -/
+@[grind]
+class Relation.Subrelation (r₁ r₂ : Relation α β) where
+  subsumption : ∀ a b, r₁ a b → r₂ a b
+
+-- 50 is taken from '<='
+infix:50 " ⊆ " => Relation.Subrelation
+
+namespace Relation
+
+theorem eq_of_subrelation_of_subrelation (forward : r₁ ⊆ r₂) (backward : r₂ ⊆ r₁) : r₁ = r₂ := by
+  funext x
+  grind
+
+grind_pattern eq_of_subrelation_of_subrelation => r₁ ⊆ r₂, r₂ ⊆ r₁
+
+macro "two_directions" : tactic => `(tactic|apply eq_of_subrelation_of_subrelation)
